venom/simulation/execEquivParamPropsScript.sml
@@ -14,7 +14,7 @@ Theorem step_inst_preserves_R:
     valid_state_rel R_ok R_term /\ R_ok s1 s2 /\
     (!x. MEM (Var x) inst.inst_operands ==>
          lookup_var x s1 = lookup_var x s2) ==>
-    lift_result R_ok R_term (step_inst inst s1) (step_inst inst s2)
+    lift_result R_ok R_term (step_inst_base inst s1) (step_inst_base inst s2)
 Proof
   ACCEPT_TAC step_inst_preserves_R_proof
 QED
